# Linear Equations - Complete Extraction Preview (v3)

---

## Concepts

### Concept 1: LINEAR EQUATIONS
**Source: image483.png**
![](docx_extracted/word/media/image483.png)

**Extracted:**
- **Title:** LINEAR EQUATIONS
- **Content:** A linear equation contains at least a variable which can only be raised to the power 1.
- **Linear examples:** $3x + 5 = 8$, $\frac{1}{2}x - 3 = 2$, $\frac{1+x}{3} = x$
- **Not linear examples:** $x^2 - 3x + 2 = 0$, $\frac{1}{x} = \sqrt{x}$, $x^3 = 8$

---

### Concept 2: SIDES OF AN EQUATION
**Source: image484.png**
![](docx_extracted/word/media/image484.png)

**Extracted:**
- **Title:** SIDES OF AN EQUATION
- **Content:** The left hand side (LHS) of an equation is on the left of the = sign. The right hand side (RHS) of an equation is on the right of the = sign.

---

### Concept 3: Solution
**Source: image485.png**
![](docx_extracted/word/media/image485.png)

**Extracted:**
- **Content:** The solution of a linear equation is the value of the variable which makes the equation true. In other words, it makes the left hand side (LHS) equal to the right hand side (RHS).

---

### Concept 4: ALGEBRAIC SOLUTION TO LINEAR EQUATIONS
**Source: image486.png**
![](docx_extracted/word/media/image486.png)

**Extracted:**
- **Content:** The following steps should be followed to solve linear equations:
- **Step 1:** Decide how the expression containing the unknown has been 'built up'.
- **Step 2:** Perform inverse operations on both sides of the equation to 'undo' how the equation is 'built up'. In this way we isolate the unknown.
- **Step 3:** Check your solution by substitution.

---

### Concept 5: Unknown on both sides
**Source: image491.png**
![](docx_extracted/word/media/image491.png)

**Extracted:**
- **Content:** If the unknown appears on both sides of the equation, we:
  - expand any brackets and collect like terms
  - move the unknown to one side of the equation and the remaining terms to the other side
  - simplify and then solve the equation

---

## Examples (with full solution steps)

### Example 1
**Source: image487.png**
![](docx_extracted/word/media/image487.png)

**Instruction:** Solve for x:

#### Part a: $4x - 1 = 7$

| Step | Extracted LaTeX | Explanation |
|------|-----------------|-------------|
| 1 | $4x - 1 = 7$ | - |
| 2 | $4x - 1 + 1 = 7 + 1$ | adding 1 to both sides |
| 3 | $4x = 8$ | - |
| 4 | $\frac{4x}{4} = \frac{8}{4}$ | divide both sides by 4 |
| 5 | $x = 2$ | - |

**Answer:** $x = 2$
**Check:** $4 \times 2 - 1 = 8 - 1 = 7$ ✓

#### Part b: $5 - 3x = 6$

| Step | Extracted LaTeX | Explanation |
|------|-----------------|-------------|
| 1 | $5 - 3x = 6$ | - |
| 2 | $5 - 3x - 5 = 6 - 5$ | subtracting 5 from both sides |
| 3 | $-3x = 1$ | - |
| 4 | $\frac{-3x}{-3} = \frac{1}{-3}$ | dividing both sides by -3 |
| 5 | $x = -\frac{1}{3}$ | - |

**Answer:** $x = -\frac{1}{3}$
**Check:** $5 - 3 \times (-\frac{1}{3}) = 5 + 1 = 6$ ✓

**Tip:** The inverse of + is - and × is ÷.

---

### Example 2
**Source: image488.png**
![](docx_extracted/word/media/image488.png)

#### Part a: $\frac{x}{5} - 3 = -1$

| Step | Extracted LaTeX | Explanation |
|------|-----------------|-------------|
| 1 | $\frac{x}{5} - 3 = -1$ | - |
| 2 | $\frac{x}{5} - 3 + 3 = -1 + 3$ | adding 3 to both sides |
| 3 | $\frac{x}{5} = 2$ | - |
| 4 | $\frac{x}{5} \times 5 = 2 \times 5$ | multiplying both sides by 5 |
| 5 | $x = 10$ | - |

**Answer:** $x = 10$
**Check:** $\frac{10}{5} - 3 = 2 - 3 = -1$ ✓

---

### Example 3
**Source: image489.png**
![](docx_extracted/word/media/image489.png)

#### Part b: $\frac{1}{5}(x - 3) = -1$

| Step | Extracted LaTeX | Explanation |
|------|-----------------|-------------|
| 1 | $\frac{1}{5}(x - 3) = -1$ | - |
| 2 | $\frac{1}{5}(x - 3) \times 5 = -1 \times 5$ | multiplying both sides by 5 |
| 3 | $x - 3 = -5$ | - |
| 4 | $x - 3 + 3 = -5 + 3$ | adding 3 to both sides |
| 5 | $x = -2$ | - |

**Answer:** $x = -2$
**Check:** $\frac{1}{5}((-2) - 3) = \frac{1}{5} \times -5 = -1$ ✓

---

### Example 4
**Source: image490.png**
![](docx_extracted/word/media/image490.png)

#### Problem: $3(2x - 5) - 2(x - 1) = 3$

| Step | Extracted LaTeX | Explanation |
|------|-----------------|-------------|
| 1 | $3(2x - 5) - 2(x - 1) = 3$ | - |
| 2 | $3 \times 2x + 3 \times (-5) - 2 \times x - 2 \times (-1) = 3$ | expanding brackets |
| 3 | $6x - 15 - 2x + 2 = 3$ | - |
| 4 | $4x - 13 = 3$ | collecting like terms |
| 5 | $4x - 13 + 13 = 3 + 13$ | adding 13 to both sides |
| 6 | $4x = 16$ | - |
| 7 | $x = 4$ | dividing both sides by 4 |

**Answer:** $x = 4$
**Check:** $3(2 \times 4 - 5) - 2(4 - 1) = 3 \times 3 - 2 \times 3 = 3$ ✓

---

### Example 5
**Source: image492.png**
![](docx_extracted/word/media/image492.png)

#### Part a: $3x - 4 = 2x + 6$

| Step | Extracted LaTeX | Explanation |
|------|-----------------|-------------|
| 1 | $3x - 4 = 2x + 6$ | - |
| 2 | $3x - 4 - 2x = 2x + 6 - 2x$ | subtracting 2x from both sides |
| 3 | $x - 4 = 6$ | - |
| 4 | $x - 4 + 4 = 6 + 4$ | adding 4 to both sides |
| 5 | $x = 10$ | - |

**Answer:** $x = 10$
**Check:** LHS = $3 \times 10 - 4 = 26$, RHS = $2 \times 10 + 6 = 26$ ✓

#### Part b: $4 - 3(2 + x) = x$

| Step | Extracted LaTeX | Explanation |
|------|-----------------|-------------|
| 1 | $4 - 3(2 + x) = x$ | - |
| 2 | $4 - 6 - 3x = x$ | expanding |
| 3 | $-2 - 3x = x$ | - |
| 4 | $-2 - 3x + 3x = x + 3x$ | adding 3x to both sides |
| 5 | $-2 = 4x$ | - |
| 6 | $\frac{-2}{4} = \frac{4x}{4}$ | dividing both sides by 4 |
| 7 | $-\frac{1}{2} = x$ | - |

**Answer:** $x = -\frac{1}{2}$
**Check:** LHS = $4 - 3(2 + (-\frac{1}{2})) = 4 - 3 \times \frac{3}{2} = 4 - 4\frac{1}{2} = -\frac{1}{2}$ = RHS ✓

---

## Exercises (problems only, no answers in original)

### EXERCISE 1C.1
**Source: image493.png**
![](docx_extracted/word/media/image493.png)

**Q1 - Solve for x:**
| a | b | c | d |
|---|---|---|---|
| $x + 9 = 4$ | $5x = 45$ | $-24 = -6x$ | $3 - x = 12$ |

| e | f | g | h |
|---|---|---|---|
| $2x + 5 = 17$ | $3x - 2 = -14$ | $3 - 4x = -17$ | $8 = 9 - 2x$ |

**Q2 - Solve for x:**
| a | b | c | d |
|---|---|---|---|
| $\frac{x}{4} = 12$ | $\frac{1}{2}x = 6$ | $5 = \frac{x}{-2}$ | $\frac{x}{3} + 4 = -2$ |

| e | f | g | h |
|---|---|---|---|
| $\frac{x+3}{5} = -2$ | $\frac{1}{3}(x+2) = 3$ | $\frac{2x-1}{3} = 7$ | $\frac{1}{2}(5-x) = -2$ |

---

### EXERCISE 1C.2
**Source: image494.png**
![](docx_extracted/word/media/image494.png)

**Q1 - Solve for x:**
| a | b | c |
|---|---|---|
| $2(x+8) + 5(x-1) = 60$ | $2(x-3) + 3(x+2) = -5$ | $3(x+3) - 2(x+1) = 0$ |

| d | e | f |
|---|---|---|
| $4(2x-3) + 2(x+2) = 32$ | $3(4x+1) - 2(3x-4) = -7$ | $5(x+2) - 2(3-2x) = -14$ |

**Q2 - Solve for x:**
| a | b | c | d | e |
|---|---|---|---|---|
| $2x - 3 = 3x + 6$ | $3x - 4 = 5 - x$ | $4 - 5x = 3x - 8$ | $-x = 2x + 4$ | $12 - 7x = 3x + 7$ |

| f | g | h | i | j |
|---|---|---|---|---|
| $5x - 9 = 1 - 3x$ | $4 - x - 2(2-x) = 6 + x$ | $5 - 3(1-x) = 2 - 3x$ | $5 - 2x - (2x+1) = -6$ | $3(4x+2) - x = -7 + x$ |

**Q3 - Solve for x:**
- a: $2(3x+1) - 3 = 6x - 1$
- b: $3(4x+1) = 6(2x+1)$
- c: Comment on your solutions to a and b.

---

### EXERCISE 6A
**Source: image495.png**
![](docx_extracted/word/media/image495.png)

**Q1 - The solution of each of the following equations is one of the given possibilities. Find the solution by trial and error.**
| | Equation | Choices |
|---|----------|---------|
| a | $2x - 9 = 5$ | {3, 5, 7} |
| b | $3 - a = -1$ | {2, 4, 6} |
| c | $\frac{x+6}{2} = 1$ | {-4, -2, 0} |
| d | $\frac{6}{1+y} = 3$ | {1, 2, 3} |

**Q2 - Which of the following equations are: A true for exactly one value of x, B true for two values of x, C true for all values of x, D never true, E true for all values of x except 0?**
| a | b | c | d | e | f |
|---|---|---|---|---|---|
| $x + 3 = 5$ | $x^2 = 0$ | $\frac{1}{x} = 0$ | $2x = 11$ | $x^2 = 9$ | $x - x = 0$ |

| g | h | i | j | k | l |
|---|---|---|---|---|---|
| $x - 1 = x$ | $2 + 5x = 12$ | $x - x^2 = 0$ | $3x \times 2x = 6x^2$ | $\frac{1}{x} \times x = 1$ | $2 - \frac{1}{x} = 3$ |

---

### EXERCISE 6D
**Q1 - Source: image496.png**
![](docx_extracted/word/media/image496.png)

**Solve for x:**
| a | b | c | d | e | f |
|---|---|---|---|---|---|
| $x + 3 = 0$ | $3x = -9$ | $3x + 6 = 0$ | $3x - 4 = -6$ | $5x + 8 = 18$ | $4x - 9 = 1$ |

| g | h | i | j | k | l |
|---|---|---|---|---|---|
| $8x - 7 = 9$ | $3x + 6 = -7$ | $6 + 7x = -1$ | $9 = 3x + 7$ | $6x - 7 = -1$ | $-1 = 2x + 6$ |

---

**Q2 - Source: image497.png**
![](docx_extracted/word/media/image497.png)

**Solve for x:**
| a | b | c | d | e | f |
|---|---|---|---|---|---|
| $6 - x = -5$ | $-4x = 15$ | $3 - 2x = 7$ | $5 - 4x = -7$ | $3 - 7x = -2$ | $17 - 2x = -1$ |

| g | h | i | j | k | l |
|---|---|---|---|---|---|
| $11 = 3 - 2x$ | $15 - 2x = -1$ | $8 = 3 - 2x$ | $6 = -1 - 7x$ | $-15 = 3 - 6x$ | $11 = -4 - 3x$ |

---

**Q3 - Source: image498.png**
![](docx_extracted/word/media/image498.png)

**Solve for x:**
| a | b | c | d | e | f |
|---|---|---|---|---|---|
| $\frac{x}{2} = 5$ | $\frac{2x}{3} = -4$ | $\frac{x}{4} + 1 = -3$ | $\frac{x}{3} - 2 = 1$ | $\frac{x-1}{2} = 1$ | $\frac{x+5}{3} = -1$ |

---

**Q4 - Source: image499.png**
![](docx_extracted/word/media/image499.png)

**Solve for x:**
| a | b | c | d | e | f |
|---|---|---|---|---|---|
| $\frac{2x+7}{5} = 0$ | $\frac{1}{2}(1-3x) = -1$ | $\frac{1+4x}{7} = 3$ | $\frac{3x-1}{2} = 4$ | $\frac{1}{5}(4-3x) = -1$ | $\frac{1}{4}(1+2x) = -2$ |

---

### EXERCISE 6E
**Q1, Q2 - Source: image500.png**
![](docx_extracted/word/media/image500.png)

**Q1 - Solve for x:**
| a | b | c | d | e | f |
|---|---|---|---|---|---|
| $4(x-1) - 2x = 2$ | $2(x-3) + 3x = 9$ | $5(x+2) - 2x = 4$ | $3(2x+3) - 4x = -3$ | $6(3x+2) - 5x = -1$ | $-4(2x-1) + 5x = -12$ |

**Q2 - Solve for x:**
| a | b | c | d | e | f |
|---|---|---|---|---|---|
| $3(x+1) + 4(x+2) = -3$ | $5(x+3) - 2(x-1) = 2$ | $4(x-2) - (x+1) = 6$ | $2(x+4) + 8(x-2) = 12$ | $3(2x+1) - 4(x+2) = 9$ | $3(5x-2) - 2(3x-4) = 2$ |

---

**Q3 - Source: image501.png**
![](docx_extracted/word/media/image501.png)

**Solve for x:**
| a | b | c | d | e | f |
|---|---|---|---|---|---|
| $3x + 2 = x + 10$ | $7x + 2 = 4x - 8$ | $8x + 3 = 4x + 4$ | $3x - 1 = 6x - 4$ | $4x - 2 = 8x + 10$ | $5 + 2x = 18 + 4x$ |

---

**Q4, Q5 - Source: image502.png**
![](docx_extracted/word/media/image502.png)

**Q4 - Solve for x:**
| a | b | c | d | e | f |
|---|---|---|---|---|---|
| $3x + 5 = 1 - x$ | $6 + 2x = 15 - x$ | $6 + x = 13 - 2x$ | $9 - 2x = 12 - 7x$ | $4 - 3x = 8 - x$ | $9 - 3x = x + 2$ |

**Q5 - Solve for x:**
| a | b | c | d | e | f |
|---|---|---|---|---|---|
| $3(x+1) - x = 15$ | $5(x+2) - 2x = 11$ | $6(1-2x) = -4 - 7x$ | $2(x+4) + 8(x-2) = 12$ | $4(3x+1) + 18 = x$ | $7x - 2(x+1) = 13$ |

| g | h | i | j | k | l |
|---|---|---|---|---|---|
| $14x - 5(2x+5) = 7$ | $19 - (3-x) = 5x$ | $2x - 4(4-3x) = x + 10$ | $2(x+4) = 7 - (3+x)$ | $2(x-6) + 7x = 3(3x-4)$ | $5(2x-4) = 4x - 2(1-3x)$ |

---

**Q6 - Source: image503.png**
![](docx_extracted/word/media/image503.png)

**Solve the following equations:**
| a | b | c | d | e | f |
|---|---|---|---|---|---|
| $3(x-2) = x + 4$ | $4(t-3) = 3 - t$ | $3(2y-1) = 4y - 5$ | $2(a+6) = 7 - 2a$ | $4(2b+3) = b + 12$ | $8(a+2) = 1 + 3a$ |

---

**Q7, Q8 - Source: image504.png**
![](docx_extracted/word/media/image504.png)

**Q7:**
- a: Try to solve $3(a+2) = 6 + 3a$. What do you notice?
- b: How many values of a satisfy the equation?

**Q8:**
- a: Try to solve $2(2a+3) = 5 + 4a$. What do you notice?
- b: How many values of a satisfy the equation?

---

**Q9, Q10 - Source: image505.png**
![](docx_extracted/word/media/image505.png)

**Q9 - Solve the following equations:**
| a | b | c | d | e | f | g |
|---|---|---|---|---|---|---|
| $2 - x = 3(x+3) + 1$ | $2x + 1 = 2(1-3x) + 7$ | $12 - x = 2(x-2) + x$ | $4 + 3p = 2 + 5(1-p)$ | $3x + 2(x+1) = 8$ | $4x - 1 + 3(2x-2) = 4$ | $x + 2 - 4(x-1) = 11$ |

| h | i | j | k | l | m | n |
|---|---|---|---|---|---|---|
| $2(x-1) - 5(x+2) = -8$ | $3(1-x) - 2(2-x) = 4$ | $5(x-2) + 3(1-2x) = 6$ | $4(2x-3) - 5(3x+1) = -2$ | $3 - 2x - (x+4) = -11$ | $2(1-3x) - (5-x) = 7$ | $4x + 2(x-1) + x = 9$ |

**Q10 - Solve the following equations:**
| a | b | c | d | e |
|---|---|---|---|---|
| $12(x-1) = 3(2x+1) + 9$ | $3(2p-1) = 5(1-p) + 3$ | $2(5x+1) + 2 = 3(x-1)$ | $6(x-4) + 2(x+5) = 3(x-1) + 4$ | $x - 5 - (2x+1) = 4x + 3$ |

| f | g | h | i | j |
|---|---|---|---|---|
| $3 - 2x = 4(x+1) - 3(1-x)$ | $4x + 2(1-x) = 5 - (1-4x)$ | $5 - (2-3x) = 11 - (5-4x)$ | $x = 3(2x-1) - 4(2-x)$ | $2(x-2) - 3(5-x) = 4(2x+1)$ |

---

### Handwritten Exercise
**Source: image506.png**
![](docx_extracted/word/media/image506.png)

**Solve all these equations!**
| # | Problem | # | Problem |
|---|---------|---|---------|
| 1 | $a - 5 = 19$ | 2 | $b + 19 = 38$ |
| 3 | $7c = 91$ | 4 | $\frac{d}{5} = 20$ |
| 5 | $11e - 5 = 72$ | 6 | $2f + 4 = 80$ |
| 7 | $g + 5g = 72$ | 8 | $3h = 90 - 2h$ |
| 9 | $3j + 2 = 27 - 2j$ | 10 | $36 - 4k = 0$ |
| 11 | $12m - 5 = 15 + 8m$ | 12 | $2n + 7 = 31 - 4n$ |
| 13 | $3(p+2) - p = 26$ | 14 | $4(2r-6) + 3(r+5) = 35$ |
| 15 | $\frac{1}{2}(t-4) = 12$ | 16 | $\frac{w+7}{5} = 5$ |
| 17 | $2(2a-5) + 4(a+7) = 82$ | 18 | $5(c+3) + (c-6) = 27$ |
| 19 | $2(e+5) - 3(6-e) = 42$ | 20 | $5(f-1) + 3(f-4) = 23$ |
| 21 | $22 - 5k - (k+10) = 0$ | 22 | $2(3m-4) - 2(m+7) = 0$ |

**Source: image507.png**
![](docx_extracted/word/media/image507.png)

| # | Problem |
|---|---------|
| 23 | $3a + 5 = 17 - a$ |
| 24 | $25 - 7c = -10$ |
| 25 | $12d - 5 = 15 + 10d$ |
| 26 | $\frac{2a-5}{3} = \frac{a-2}{2}$ |
| 27 | $\frac{c-1}{3} = c - \frac{3(c+2)}{5}$ |
| 28 | $5n - 2 = n - 3(n+3)$ |

---

## Summary

| Type | Count |
|------|-------|
| Concepts | 5 |
| Examples (with full solutions) | 7 problems |
| Exercise questions | ~170 problems |

**Please verify by comparing original images with extracted content!**
